src/ecTyping.ml
@@ -1533,11 +1533,23 @@ let trans_form_or_pattern env (ps, ue) pf tt =
           | None -> tyerror x.pl_loc env (UnknownVarOrOp (unloc x, []))
           | Some (x, ty) -> f_pvar x ty me
         in
-
-        let xs1 = List.map (lookup EcFol.mleft ) xs in
-        let xs2 = List.map (lookup EcFol.mright) xs in
-        let eqs = List.map2 (fun x1 x2 -> f_eq x1 x2) xs1 xs2 in
-
+        let check_mem loc me = 
+          match EcEnv.Memory.byid me env with
+          | None -> tyerror loc env NoActiveMemory (* FIXME error message *)
+          | Some _ -> () in
+        let do1 = function
+          | GVvar x ->
+            let x1 = lookup EcFol.mleft x in
+            let x2 = lookup EcFol.mright x in
+            f_eq x1 x2
+          | GVglob gp ->
+            let mp = trans_topmsymbol env gp in
+            check_mem gp.pl_loc EcFol.mleft;
+            check_mem gp.pl_loc EcFol.mright;
+            let x1 = f_glob mp EcFol.mleft in
+            let x2 = f_glob mp EcFol.mright in
+            f_eq x1 x2 in
+        let eqs = List.map do1 xs in
         EcFol.f_ands eqs
 
     | PFapp ({pl_desc = PFident ({ pl_desc = name; pl_loc = loc }, tvi)}, es) ->
