examples/elgamal.ec
@@ -234,11 +234,11 @@ proof.
  fun.
  inline ElGamal.kg ElGamal.enc Inv(A).inv.
  wp.
- call (={c} /\ (glob A){1} = (glob A){2}) (={res} /\ (glob A){1} = (glob A){2}).
+ call (={c, glob A}) (={res, glob A}).
  fun true;try (simplify;split).
  swap{1} 7 -5. 
  wp;rnd.
- call (={pk}) (={res} /\ (glob A){1} = (glob A){2}).
+ call (={pk}) (={res, glob A}).
  fun true;try (simplify;split).
  wp; do rnd; skip. simplify; smt. 
 
@@ -270,11 +270,10 @@ proof.
  equiv_deno (_: true ==> ={res});trivial.
   fun. inline{2} Inv(A).inv.
   swap{1} 7 -4;wp.
-  call (={c} /\ (glob A){1} = (glob A){2})
-      (={res} /\ (glob A){1} = (glob A){2}).
+  call (={c,glob A}) (={res,glob A}).
     fun true;try (simplify;split).
   wp;rnd.
-  call (={pk}) (={res} /\ (glob A){1} = (glob A){2}).
+  call (={pk}) (={res,glob A}).
     fun true;try (simplify;split).
   wp;do rnd;skip;by trivial. 
 save.
@@ -285,13 +284,13 @@ proof.
  equiv_deno (_: true ==> ={res});try trivial.
  fun. 
  swap{2} 10 -4;wp.
- call (={c} /\ (glob A){1} = (glob A){2})
-      (={res} /\ (glob A){1} = (glob A){2}).
+ call (={c,glob A})
+      (={res,glob A}).
     fun true;try (simplify;split).
  wp; rnd (lambda (z:int), (z + log(if b then m1 else m0){2}) %% q)
      (lambda (z:int), (z - log(if b then m1 else m0){2}) %% q).
  wp;rnd;simplify.
- call (={pk}) (={res} /\ (glob A){1} = (glob A){2}).
+ call (={pk}) (={res,glob A}).
    fun true;try (simplify;split).
  wp;do rnd;skip; progress; smt.
 save.
@@ -308,21 +307,15 @@ proof.
  conseq  (_ : ==> true) .
  intros &m;progress.
  apply (Dbool.mu_x_def (b'{m})).
- call (true) (true).
- apply Ha2.
- wp.
+ call (true) (true);try assumption.
+ cut H1 : mu [0..Int.(-) q 1] Fun.cpTrue = 1%r by smt.
+ wp; rnd (1%r) Fun.cpTrue.
+ conseq (_ : _ ==> true);[assumption | ].
+ call (true) (true);[assumption | ].
+ wp; rnd (1%r) Fun.cpTrue.
+ conseq (_ : _ ==> true);[trivial | ].
  rnd (1%r) Fun.cpTrue.
- conseq (_ : _ ==> true).
- smt.
- call (true) (true).
- apply Ha1.
- wp.
- rnd (1%r) Fun.cpTrue.
- conseq (_ : _ ==> true).
- smt.
- rnd (1%r) Fun.cpTrue.
- conseq (_ : _ ==> true).
- smt.
+ conseq (_ : _ ==> true);[trivial | ].
  skip;trivial.
 save.
 
